txn-data-consistency/EP+_TCCv_proof.thy
@@ -1746,6 +1746,21 @@ next
   qed (auto simp add: CO_Tn_is_Cmt_Abs_def tps_trans_defs)
 qed
 
+definition CO_is_Cmt_Abs where
+  "CO_is_Cmt_Abs s k \<longleftrightarrow> (\<forall>t. t \<in> set (commit_order s k) \<longrightarrow>
+    (\<exists>cts v rs deps. svr_state (svrs s k) t = Commit cts v rs deps) \<or> 
+    ((\<exists>ts v. svr_state (svrs s k) t = Prep ts v) \<and> 
+     (\<exists>cts kv_map deps. cl_state (cls s (get_cl_w t)) = WtxnCommit cts kv_map deps \<and> k \<in> dom kv_map)))"
+
+lemmas CO_is_Cmt_AbsI = CO_is_Cmt_Abs_def[THEN iffD2, rule_format]
+lemmas CO_is_Cmt_AbsE[elim] = CO_is_Cmt_Abs_def[THEN iffD1, elim_format, rule_format]
+
+lemma reach_co_is_cmt_abs [simp]: "reach tps s \<Longrightarrow> CO_is_Cmt_Abs s k"
+  apply (simp add: CO_is_Cmt_Abs_def)
+  apply rule subgoal for t apply (cases t)
+    apply (metis Init_Ver_Inv_def reach_init_ver_inv)
+    by (metis (lifting) CO_Tn_is_Cmt_Abs_def get_cl_w.simps(2) reach_co_tn_is_cmt_abs txid0.exhaust).
+
 definition CO_not_No_Ver where
   "CO_not_No_Ver s k \<longleftrightarrow> (\<forall>t \<in> set (commit_order s k). svr_state (svrs s k) t \<noteq> No_Ver)"
 
@@ -1753,11 +1768,8 @@ lemmas CO_not_No_VerI = CO_not_No_Ver_def[THEN iffD2, rule_format]
 lemmas CO_not_No_VerE[elim] = CO_not_No_Ver_def[THEN iffD1, elim_format, rule_format]
 
 lemma reach_co_not_no_ver [simp]: "reach tps s \<Longrightarrow> CO_not_No_Ver s k"
-  apply (simp add: CO_not_No_Ver_def)
-  apply rule subgoal for t apply (cases t)
-     apply (metis Init_Ver_Inv_def reach_init_ver_inv ver_state.distinct(3))
-    using CO_Tn_is_Cmt_Abs_def
-    by (metis reach_co_tn_is_cmt_abs txid0.exhaust ver_state.distinct(1) ver_state.distinct(3)).
+  apply (auto simp add: CO_not_No_Ver_def)
+  by (metis CO_is_Cmt_Abs_def reach_co_is_cmt_abs ver_state.distinct(1) ver_state.distinct(3))
 
 definition CO_has_Cts where
   "CO_has_Cts s k \<longleftrightarrow> (\<forall>t \<in> set (commit_order s k). \<exists>cts. wtxn_cts s t = Some cts)"
@@ -2110,6 +2122,37 @@ next
   qed (auto simp add: Rtxn_RegK_in_rs_def tps_trans_defs)
 qed
 
+definition Rtxn_notin_rs_other_t where
+  "Rtxn_notin_rs_other_t s cl \<longleftrightarrow> (\<forall>k keys kvt_map t cts v rs deps t'.
+    cl_state (cls s cl) = RtxnInProg keys kvt_map \<and> kvt_map k = Some (v, t) \<and> t' \<noteq> t \<and>
+    svr_state (svrs s k) t' = Commit cts v rs deps \<longrightarrow> get_txn s cl \<notin> rs)"
+
+lemmas Rtxn_notin_rs_other_tI = Rtxn_notin_rs_other_t_def[THEN iffD2, rule_format]
+lemmas Rtxn_notin_rs_other_tE[elim] = Rtxn_notin_rs_other_t_def[THEN iffD1, elim_format, rule_format]
+
+lemma reach_rtxn_notin_rs_other_t [simp]: "reach tps s \<Longrightarrow> Rtxn_notin_rs_other_t s cl"
+proof(induction s rule: reach.induct)
+  case (reach_init s)
+  then show ?case by (auto simp add: Rtxn_notin_rs_other_t_def tps_defs)
+next
+  case (reach_trans s e s')
+  then show ?case 
+  proof (induction e)
+    case (Read x1 x2 x3 x4)
+    then show ?case apply (auto simp add: Rtxn_notin_rs_other_t_def tps_trans_defs
+          split: if_split_asm, auto) using Rtxn_IdleK_notin_rs_def[of s x1] sorry
+  next
+    case (RegR x1 x2 x3 x4)
+    then show ?case by (auto simp add: Rtxn_notin_rs_other_t_def tps_trans_defs
+          add_to_readerset_def split: ver_state.split, blast+)
+  next
+    case (PrepW x1 x2 x3)
+    then show ?case by (simp add: Rtxn_notin_rs_other_t_def tps_trans_defs, blast)
+  next
+    case (CommitW x1 x2 x3 x4 x5)
+    then show ?case by (simp add: Rtxn_notin_rs_other_t_def tps_trans_defs, blast)
+  qed (auto simp add: Rtxn_notin_rs_other_t_def tps_trans_defs)
+qed
 
 subsection \<open>Timestamp relations\<close>
 
@@ -2146,7 +2189,7 @@ next
   qed (auto simp add: Disjoint_RW_def tps_trans_defs)
 qed
 
-definition Disjoint_RW' where
+(*definition Disjoint_RW' where
   "Disjoint_RW' s \<longleftrightarrow> (kvs_writers (kvs_of_s s) \<inter> Tn ` kvs_readers (kvs_of_s s) = {})"
 
 lemmas Disjoint_RW'I = Disjoint_RW'_def[THEN iffD2, rule_format]
@@ -2186,7 +2229,7 @@ next
     case (WCommit x1 x2 x3 x4 x5)
     then show ?case sorry
   qed (auto simp add: Disjoint_RW'_def)
-qed
+qed*)
 
 definition RO_has_rts where
   "RO_has_rts s \<longleftrightarrow> (\<forall>t. Tn t \<in> read_only_Txs (kvs_of_s s) \<longrightarrow> (\<exists>rts. rtxn_rts s t = Some rts))"
